wip

specs/Spec.Chacha20_vec.fst
@@ -27,13 +27,13 @@ type state = m:seq vec      {length m = 4}
 type idx = n:nat{n < 4}
 type shuffle = state -> Tot state 
 
-unfold let op_Plus_Percent_Hat (x:vec) (y:vec) : Tot vec = 
+(* unfold  *)let op_Plus_Percent_Hat (x:vec) (y:vec) : Tot vec = 
        Combinators.seq_map2 U32.op_Plus_Percent_Hat x y
 
-unfold let op_Hat_Hat (x:vec) (y:vec) : Tot vec = 
+(* unfold *) let op_Hat_Hat (x:vec) (y:vec) : Tot vec = 
        Combinators.seq_map2 U32.op_Hat_Hat x y
 
-unfold let op_Less_Less_Less (x:vec) (n:UInt32.t{v n < 32}) : Tot vec = 
+(* unfold *) let op_Less_Less_Less (x:vec) (n:UInt32.t{v n < 32}) : Tot vec = 
        Combinators.seq_map (fun x -> x <<< n) x 
 
 let shuffle_right (x:vec) (n:idx) : Tot vec =
@@ -51,61 +51,53 @@ let shuffle_right (x:vec) (n:idx) : Tot vec =
 let shuffle_row (i:idx) (n:idx) (s:state) : Tot state = 
        upd s i (shuffle_right (index s i) n)
 
-val line: idx -> idx -> idx -> s:UInt32.t {v s < 32} -> shuffle
+val line: idx -> idx -> idx -> s:UInt32.t {v s < 32} -> st:state -> Tot state
 let line a b d s m = 
   let m = upd m a (index m a +%^ index m b) in
   let m = upd m d ((index m d ^^  index m a) <<< s) in
   m
 
 
-let round : shuffle =
-  line 0 1 3 16ul @
-  line 2 3 1 12ul @
-  line 0 1 3 8ul  @
-  line 2 3 1 7ul
+let round (st:state) : Tot state =
+  let st = line 0 1 3 16ul st in
+  let st = line 2 3 1 12ul st in
+  let st = line 0 1 3 8ul  st in
+  let st = line 2 3 1 7ul  st in
+  st
 
 
-let shuffle_rows_0123 : shuffle =
-  shuffle_row 1 1 @
-  shuffle_row 2 2 @
-  shuffle_row 3 3
+let shuffle_rows_0123 (st:state) : Tot state =
+  let st = shuffle_row 1 1 st in
+  let st = shuffle_row 2 2 st in
+  let st = shuffle_row 3 3 st in
+  st
 
 
-let shuffle_rows_0321 : shuffle =
-  shuffle_row 1 3 @
-  shuffle_row 2 2 @
-  shuffle_row 3 1
+let shuffle_rows_0321 (st:state) : Tot state =
+  let st = shuffle_row 1 3 st in
+  let st = shuffle_row 2 2 st in
+  let st = shuffle_row 3 1 st in
+  st
 
 
-let column_round : shuffle = round
+let column_round (st:state) : Tot state = round st
 
 
-let diagonal_round : shuffle =
-  shuffle_rows_0123 @
-  round           @
-  shuffle_rows_0321
+let diagonal_round (st:state) : Tot state =
+  let st = shuffle_rows_0123 st in
+  let st = round           st in
+  let st = shuffle_rows_0321 st in
+  st
 
 
-let double_round : shuffle =
-  column_round @ diagonal_round
-  (* line 0 1 3 16ul @ *)
-  (* line 2 3 1 12ul @ *)
-  (* line 0 1 3 8ul  @ *)
-  (* line 2 3 1 7ul  @ *)
-  (* shuffle_row 1 1 @ *)
-  (* shuffle_row 2 2 @ *)
-  (* shuffle_row 3 3 @ *)
-  (* line 0 1 3 16ul @ *)
-  (* line 2 3 1 12ul @ *)
-  (* line 0 1 3 8ul  @ *)
-  (* line 2 3 1 7ul  @ *)
-  (* shuffle_row 1 3 @ *)
-  (* shuffle_row 2 2 @ *)
-  (* shuffle_row 3 1 *)
+let double_round (st:state) : Tot state =
+  let st = column_round st in
+  let st = diagonal_round st in
+  st
 
 
-let rounds : shuffle = 
-    iter 10 double_round (* 20 rounds *)
+let rounds (st:state) : Tot state = 
+    iter 10 double_round st (* 20 rounds *)
 
 let chacha20_core (s:state) : Tot state = 
     let s' = rounds s in
